src/tactics/FStar.Tactics.Interpreter.fst
@@ -423,6 +423,10 @@ let () =
         pack_curried    RE.e_term_view RE.e_term
         pack_curried    NRE.e_term_view NRE.e_term;
 
+      mk_tac_step_1 0 "bv_ppname"
+        bv_ppname       RE.e_bv e_string
+        bv_ppname       NRE.e_bv NBET.e_string;
+
       mk_tac_step_1 0 "fresh"
         fresh       e_unit e_int
         fresh       NBET.e_unit NBET.e_int;
